Typeclass-based maps for easier proving later.

LambdaS5/caml/PrettyPrint.ml
@@ -30,7 +30,7 @@ and string_of_object depth (st : store) obj =
   (string_of_value depth st (object_proto obj)) (String.of_list (object_class obj))
   (object_extensible obj) (string_of_value depth st (object_prim_value obj))
   (string_of_value depth st (object_code obj))
-  (string_of_prop_list depth st (HeapUtils.Heap.to_list (object_properties obj)) [])
+  (string_of_prop_list depth st (LibFinmap.FinmapImpl.to_list LibOrder.Build_Lt (object_properties obj)) [])
 and string_of_prop_list depth st l skip =
   let string_of_prop = function (name, attr) ->
     Printf.sprintf "'%s': %s" (String.of_list name) (string_of_attr depth st attr)
@@ -60,7 +60,7 @@ and string_of_attr depth st = function
 | Coq_attributes_accessor_of d -> attributes_accessor_rect (fun g s e c -> Printf.sprintf "{#getter %s, #setter %s}" (string_of_value depth st g) (string_of_value depth st s)) d (* enumerable and configurable ignored *)
 
 let string_of_store depth c st =
-  let locs = Utils.Heap.to_list c in
+  let locs = LibFinmap.FinmapImpl.to_list LibOrder.Build_Lt c in
   let pred = string_of_value depth st in
   String.concat "" (List.map (fun (k, v) -> Printf.sprintf "let (%s = %s) \n" (String.of_list k) (pred v)) locs)
 
