LambdaS5/coq/LibFinmap.v
@@ -1,0 +1,129 @@
+Require Import LibTactics LibList LibListSorted.
+Require Import LibSet LibLogic LibEqual LibReflect LibOrder LibRelation.
+Generalizable Variable A R B.
+
+Import ListNotations.
+Open Scope list_scope.
+
+(* TODO utitities *)
+Definition rel_fst {A B} (R : binary A) : binary (A * B) := fun x y => R (fst x) (fst y).
+
+Class BagReadOption A B T := { read_option : T -> A -> option B }. 
+
+Notation "m \( x ?)" := (read_option m x)
+  (at level 33, format "m \( x ?)") : container_scope.
+
+Module Type FinmapSig.
+Section Definitions. 
+
+Variables (A B : Type) (LTA : Lt A).
+
+Parameter finmap : forall (A B : Type) {LTA : Lt A}, Type.
+
+Set Implicit Arguments.
+
+Parameter from_list : list (A * B) -> finmap A B.
+Parameter to_list : finmap A B -> list (A * B).
+
+Parameter empty_impl : finmap A B.
+Parameter single_bind_impl : A -> B -> finmap A B.
+Parameter in_impl : A -> finmap A B -> Prop.
+Parameter binds_impl : finmap A B -> A -> B -> Prop.
+Parameter read_impl : Inhab B -> finmap A B -> A -> B.
+Parameter read_option_impl : finmap A B -> A -> option B.
+Parameter remove_impl : finmap A B -> A -> finmap A B.
+Parameter update_impl : finmap A B -> A -> B -> finmap A B.
+
+End Definitions.
+End FinmapSig.
+
+Module Export FinmapImpl : FinmapSig.
+Section Definitions.
+
+Variables (A B : Type).
+Context {LTA : Lt A}.
+Context {IB : Inhab B}.
+Context {ST : Lt_strict_total_order }.
+
+Inductive finmap_i := finmap_intro {
+    finmap_list : list (A * B);
+    finmap_sorted : sorted (rel_fst lt) finmap_list 
+}.
+
+Definition finmap := finmap_i.
+
+Implicit Types k : A.
+Implicit Types x : B.
+Implicit Types M : finmap.
+
+
+Definition to_list := finmap_list.
+Definition from_list (l : list (A * B)) : finmap.
+Admitted.
+
+Definition empty_impl : finmap := finmap_intro nil (sorted_nil _).
+Definition single_bind_impl k x : finmap := finmap_intro [(k, x)] (sorted_one _ _).
+Definition in_impl k M : Prop := exists x, Assoc k x (finmap_list M).
+Definition binds_impl M k x : Prop := Assoc k x (finmap_list M).
+Definition read_option_impl M k : option B.
+Admitted.
+Definition read_impl M k : B := LibList.assoc k (finmap_list M).
+Program Definition remove_impl M k : finmap := finmap_intro (remove_assoc k (finmap_list M)) _.
+Obligation 1.
+Admitted. 
+Definition update_impl M k x : finmap.
+Admitted.
+
+End Definitions.
+End FinmapImpl.
+
+Section Instances.
+
+Variables (A B : Type).
+Context {LTA : Lt A}.
+Context {IB : Inhab B}.
+Context {ST : Lt_strict_total_order }.
+
+Global Instance empty_inst : BagEmpty (finmap A B) :=
+    { empty := @empty_impl _ _ _ }.
+
+Global Instance single_bind_inst : Lt_strict_total_order -> BagSingleBind A B (finmap A B) :=
+    { single_bind := @single_bind_impl _ _ _ }.
+
+Global Instance in_inst : BagIn A (finmap A B) :=
+    { is_in := @in_impl _ _ _ }.
+
+Global Instance binds_inst : BagBinds A B (finmap A B) :=
+    { binds := @binds_impl _ _ _ }.
+
+Global Instance read_inst : BagRead A B (finmap A B) :=
+    { read := @read_impl _ _ _ _ }.
+
+Global Instance read_option_inst : BagReadOption A B (finmap A B) :=
+    { read_option := @read_option_impl _ _ _ }.
+
+Global Instance remove_inst : BagRemove (finmap A B) A :=
+    { remove := @remove_impl _ _ _ }.
+
+Global Instance write_inst : BagUpdate A B (finmap A B) :=
+    { update := @update_impl _ _ _ }.
+
+End Instances.
+
+(* Extraction.
+ * Ordering relation is ignored, because it does not extracts well.
+ * Fortunately, hiding the implementation does not allow to actually observe the order.
+ * Ordering is used on Coq side only for extensionality's sake. *)
+
+Extraction Language Ocaml.
+
+Extract Constant FinmapImpl.finmap "'A" "'B" => "('A, 'B) BatMap.t". 
+Extract Constant FinmapImpl.from_list => "fun _ l -> BatMap.of_enum (BatList.enum l)".
+Extract Constant FinmapImpl.to_list => "fun _ m -> BatMap.bindings m".
+Extract Constant FinmapImpl.empty_impl => "fun _ -> BatMap.empty".
+Extract Constant FinmapImpl.single_bind_impl => "fun _ k x -> BatMap.singleton k x".
+Extract Constant FinmapImpl.read_impl => "fun _ m k -> BatMap.find k m".
+Extract Constant FinmapImpl.read_option_impl => "fun _ m k -> try Some (BatMap.find k m) with Not_found -> None".
+Extract Constant FinmapImpl.remove_impl => "fun _ m k -> BatMap.remove k m".
+Extract Constant FinmapImpl.update_impl => "fun _ m k x -> BatMap.add k x m".
+
