LambdaS5/coq/LjsExtraction.v
@@ -264,3 +264,4 @@ Extract Constant JsSyntax.env_loc_global_env_record => "0".
 Extraction Blacklist String List Bool.
 
 Separate Extraction EjsToLjs EjsFromJs LjsInterpreter LjsValues LjsSyntax LjsCommon LjsStore LjsMonads JsNumber.to_string.
+
