LambdaS5/coq/LjsOperators.v
@@ -305,7 +305,6 @@ Definition has_own_property store v1 v2 :=
   end
 .
       
-
 Definition prop_to_obj store v1 v2 :=
   let make_attr := (fun x => attributes_data_of (attributes_data_intro x false false false)) in
   match (v1, v2) with
@@ -313,18 +312,18 @@ Definition prop_to_obj store v1 v2 :=
     assert_get_object_from_ptr store ptr (fun obj =>
       match (get_object_property obj s) with
       | Some (attributes_data_of (attributes_data_intro val writ enum config)) =>
-        let props := Heap.write Heap.empty "configurable" (make_attr (bool_to_value config)) in
-        let props := Heap.write props "enumerable" (make_attr (bool_to_value enum)) in
-        let props := Heap.write props "writable" (make_attr (bool_to_value writ)) in
-        let props := Heap.write props "value" (make_attr val) in
+        let props := \{} \("configurable" := make_attr (bool_to_value config))
+                         \("enumerable" := make_attr (bool_to_value enum)) 
+                         \("writable" := make_attr (bool_to_value writ)) 
+                         \("value" := make_attr val) in
         let obj := object_intro (oattrs_intro value_undefined "Object" false value_undefined value_null) props in
         let (store, loc) := add_object store obj in
         result_some loc
       | Some (attributes_accessor_of (attributes_accessor_intro get set enum config)) =>
-        let props := Heap.write Heap.empty "configurable" (make_attr (bool_to_value config)) in
-        let props := Heap.write props "enumerable" (make_attr (bool_to_value enum)) in
-        let props := Heap.write props "setter" (make_attr set) in
-        let props := Heap.write props "getter" (make_attr get) in
+        let props := \{} \("configurable" := make_attr (bool_to_value config)) 
+                         \("enumerable" := make_attr (bool_to_value enum)) 
+                         \("setter" := make_attr set) 
+                         \("getter" := make_attr get) in
         let obj := object_intro (oattrs_intro value_undefined "Object" false value_undefined value_null) props in
         let (store, loc) := add_object store obj in
         result_some loc
