LambdaS5/coq/LjsStore.v
@@ -13,13 +13,13 @@ Implicit Type obj : object.
 
 (* LambdaJS environment storage. *)
 Definition narrow_ctx c s := 
-  ctx_intro (List.fold_left (fun cc (i : string) => Heap.write cc i (Heap.read (value_heap c) i)) (Fset.to_list s) (Heap.empty)).
+  ctx_intro (List.fold_left (fun cc (i : string) => cc \( i := value_heap c \( i ))) (LibFinset.to_list s) \{}).
 
 Definition add_object st obj : (store * value) :=
   match st with
   | store_intro obj_heap (ptr ::: stream) =>
     ((store_intro
-      (Heap.write obj_heap ptr obj)
+      (obj_heap \( ptr := obj))
       stream
     ), (value_object ptr))
   end
@@ -29,7 +29,7 @@ Definition add_closure c recid args body : value :=
     | Some i => expr_fv (expr_lambda args body) \-- i
     | None => expr_fv (expr_lambda args body) 
     end in
-  value_closure (closure_intro (Heap.to_list (value_heap (narrow_ctx c si))) recid args body)
+  value_closure (closure_intro (FinmapImpl.to_list (value_heap (narrow_ctx c si))) recid args body)
 .
 
 (* Adds function arguments to the lexical environment *)
@@ -43,35 +43,35 @@ Definition add_parameters (closure_env : ctx) (args_name : list id) (args : list
 
 Definition closure_ctx clo args :=
   let 'closure_intro c rid args_name _ := clo in
-  let c' := fold_left (fun (p : string * value) h => let (s, v) := p in Heap.write h s v) Heap.empty c in
+  let c' := fold_left (fun (p : string * value) h => let (s, v) := p in h \( s := v )) \{} c in
   let c'' := match rid with
-    | Some i => ctx_intro (Heap.write c' i (value_closure clo))
+    | Some i => ctx_intro (c' \( i := value_closure clo))
     | None => ctx_intro c'
     end in
   add_parameters c'' args_name args.
 
 Definition add_value c i v :=
   match c with
-  | ctx_intro val_heap => ctx_intro (Heap.write val_heap i v)
+  | ctx_intro val_heap => ctx_intro (val_heap \( i := v ))
   end
 .
 
 Definition update_object st ptr obj : store :=
   (* TODO: Remove the old object from the Heap (or fix LibHeap to prevent duplicates) *)
   match st with
-  | store_intro obj_heap stream => (store_intro (Heap.write obj_heap ptr obj) stream)
+  | store_intro obj_heap stream => (store_intro (obj_heap \( ptr := obj)) stream)
   end
 .
 
 Definition get_object st ptr : option object :=
-  Heap.read_option (object_heap st) ptr
+  object_heap st \( ptr ?)
 .
 Definition get_value c i : option value :=
-  Heap.read_option (value_heap c) i
+  value_heap c \( i ?)
 .
 
 Definition num_objects st : nat :=
-  List.length (Heap.to_list (object_heap st)).
+  List.length (FinmapImpl.to_list (object_heap st)).
 
 Definition ctx_of_obj_aux (o : option ctx) (p : string * attributes) : option ctx  :=
   match o with
@@ -86,20 +86,20 @@ Definition ctx_of_obj_aux (o : option ctx) (p : string * attributes) : option ct
 .
 
 Definition ctx_of_obj obj : option ctx :=
-  List.fold_left ctx_of_obj_aux (Heap.to_list (object_properties obj)) (Some create_ctx)
+  List.fold_left ctx_of_obj_aux (FinmapImpl.to_list (object_properties obj)) (Some create_ctx)
 .
 
 (* predicates for store lookup *)
 
 Definition object_binds st ptr obj :=
-    Heap.binds (object_heap st) ptr obj.
+    binds (object_heap st) ptr obj.
 
 Definition object_indom st ptr :=
-    Heap.indom (object_heap st) ptr.
+    ptr \in object_heap st.
 
 Definition id_binds c i loc :=
-    Heap.binds (value_heap c) i loc.
+    binds (value_heap c) i loc.
 
 Definition id_indom c i :=
-    Heap.indom (value_heap c) i.
+    i \in value_heap c.
 
