LambdaS5/coq/LjsValues.v
@@ -1,16 +1,10 @@
 Require Import Utils.
 Require Import String.
 Require Import JsNumber.
+Require Import LjsShared.
+Require Import LjsSyntax.
 Open Scope list_scope.
 Open Scope string_scope.
-
-Module Heap := HeapUtils.Heap.
-
-
-
-
-Require Import LjsSyntax.
-
 
 (* LambdaJS values and objects *)
 
@@ -55,28 +49,28 @@ Fixpoint name_in_list (name : prop_name) (names : list prop_name) : bool :=
 .
 
 Definition get_object_property (object : object) (name : prop_name) : option attributes :=
-  Heap.read_option (object_properties object) name
+  object_properties object \( name ?)
 .
 Definition set_object_property (obj : object) (name : prop_name) (attrs : attributes) : object :=
-  let 'object_intro ps props := obj in object_intro ps (Heap.write props name attrs)   
+  let 'object_intro ps props := obj in object_intro ps (props \( name :=  attrs))   
 .
 Definition delete_object_property (obj : object) (name : prop_name) : object :=
-  let 'object_intro ps props := obj in object_intro ps (Heap.rem props name) 
+  let 'object_intro ps props := obj in object_intro ps (props \- name) 
 .
 
 Definition make_prop_list_aux (left : nat * object_props) (val : string) : nat * object_props :=
   match left with
   | (nb_entries, attrs) =>
     let attr := attributes_data_of (attributes_data_intro (value_string val) false false false) in
-    (S nb_entries, Heap.write attrs (Utils.string_of_nat nb_entries) attr)
+    (S nb_entries, attrs \(Utils.string_of_nat nb_entries := attr))
   end
 .
 Definition make_prop_list obj : object :=
-  match List.fold_left make_prop_list_aux (List.map fst (Heap.to_list (object_properties obj))) (0, Heap.empty) with
+  match List.fold_left make_prop_list_aux (List.map fst (FinmapImpl.to_list (object_properties obj))) (0, \{}) with
   | (nb_entries, attrs) =>
     let length := value_number (JsNumber.of_int nb_entries) in
     let length_attr := attributes_data_of (attributes_data_intro length false false false) in
-    let props := Heap.write attrs "length" length_attr in
+    let props := attrs \( "length" := length_attr ) in
     {| 
       object_attrs := {|
         oattrs_proto := value_null;
